coq/DSigmaHCOL/DSigmaHCOL.v
@@ -35,12 +35,12 @@ Module Type MDSigmaHCOL (Import CT: CType) (Import NT: NType).
   Inductive DSHVal :=
   | DSHnatVal (n:NT.t): DSHVal
   | DSHCTypeVal (a:CT.t): DSHVal
-  | DSHPtrVal (a:mem_block_id) (size:nat): DSHVal.
+  | DSHPtrVal (a:mem_block_id) (size:NT.t): DSHVal.
 
   Inductive DSHValType: DSHVal -> DSHType -> Prop :=
   | DSHnatVal_type (n:NT.t): DSHValType (DSHnatVal n) DSHnat
   | DSHCTypeVal_type (a:CT.t): DSHValType (DSHCTypeVal a) DSHCType
-  | DSHDSHPtrVal_type (a:mem_block_id) (size:nat): DSHValType (DSHPtrVal a size) (DSHPtr).
+  | DSHDSHPtrVal_type (a:mem_block_id) (size:NT.t): DSHValType (DSHPtrVal a size) (DSHPtr).
 
   (* Functional version. *)
   Definition DSHValToType: DSHVal -> DSHType :=
@@ -58,7 +58,7 @@ Module Type MDSigmaHCOL (Import CT: CType) (Import NT: NType).
     destruct v; constructor.
   Qed.
 
-  (* Expressions which evaluate to `nat` *)
+  (* Expressions which evaluate to `NT.t` *)
   Inductive NExpr : Type :=
   | NVar  : var_id -> NExpr
   | NConst: NT.t -> NExpr
@@ -107,9 +107,9 @@ Module Type MDSigmaHCOL (Import CT: CType) (Import NT: NType).
   | DSHMemMap2 (n: nat) (x0_p x1_p y_p: PExpr) (f: AExpr) (* No direct correspondance in SHCOL *)
   | DSHPower (n:NExpr) (src dst: MemVarRef) (f: AExpr) (initial: CT.t) (* formely [Inductor] *)
   | DSHLoop (n:nat) (body: DSHOperator) (* Formerly [IUnion] *)
-  | DSHAlloc (size:nat) (body: DSHOperator) (* allocates new uninitialized memory block and puts pointer to it on stack. The new block will be visible in the scope of [body] *)
-  | DSHMemInit (size:nat) (y_p: PExpr) (value: CT.t) (* Initialize memory block indices [0-size] with given value *)
-  | DSHMemCopy (size:nat) (x_p y_p: PExpr)(* copy memory blocks. Overwrites output block values, if present *)
+  | DSHAlloc (size:NT.t) (body: DSHOperator) (* allocates new uninitialized memory block and puts pointer to it on stack. The new block will be visible in the scope of [body] *)
+  | DSHMemInit (size:NT.t) (y_p: PExpr) (value: CT.t) (* Initialize memory block indices [0-size] with given value *)
+  | DSHMemCopy (size:NT.t) (x_p y_p: PExpr)(* copy memory blocks. Overwrites output block values, if present *)
   | DSHSeq (f g: DSHOperator) (* execute [g] after [f] *)
   .
 
@@ -134,7 +134,7 @@ Module Type MDSigmaHCOL (Import CT: CType) (Import NT: NType).
   Inductive DSHVal_equiv: DSHVal -> DSHVal -> Prop :=
   | DSHnatVal_equiv {n0 n1:NT.t}: n0=n1 -> DSHVal_equiv (DSHnatVal n0) (DSHnatVal n1)
   | DSHCTypeVal_equiv {a b: CT.t}: a=b -> DSHVal_equiv (DSHCTypeVal a) (DSHCTypeVal b)
-  | DSHPtr_equiv {p0 p1: mem_block_id} {s0 s1:nat}: s0 ≡ s1 /\ p0=p1 -> DSHVal_equiv (DSHPtrVal p0 s0) (DSHPtrVal p1 s1).
+  | DSHPtr_equiv {p0 p1: mem_block_id} {s0 s1:NT.t}: s0 = s1 /\ p0=p1 -> DSHVal_equiv (DSHPtrVal p0 s0) (DSHPtrVal p1 s1).
 
   Instance DSHVar_Equivalence:
     Equivalence DSHVal_equiv.
@@ -440,14 +440,14 @@ Module Type MDSigmaHCOL (Import CT: CType) (Import NT: NType).
                    string_of_nat n ++ " "
       | DSHAlloc size body =>
         "DSHAlloc " ++
-                    string_of_nat size
+                    NT.to_string size
       | DSHMemInit size y_p value =>
         "DSHMemInit " ++
-                      string_of_nat size ++ " " ++
+                      NT.to_string size ++ " " ++
                       string_of_PExpr y_p ++ " ..."
       | DSHMemCopy size x_p y_p =>
         "DSHMemCopy " ++
-                      string_of_nat size ++ " " ++
+                      NT.to_string size ++ " " ++
                       string_of_PExpr x_p ++ " " ++
                       string_of_PExpr y_p ++ " ..."
       | DSHSeq f g => "DSHSeq"
